Diagrams can have negated and transitive-closure links and still "work".

examples/lambda/diagsScript.sml
@@ -2,29 +2,47 @@ open HolKernel Parse boolLib
 
 open relationTheory bossLib boolSimps
 
+open pred_setTheory
+
 val _ = new_theory "diags"
 
+(* Diagram evaluation *)
+val _ = Hol_datatype `reltype = Atomic | TC`
+
+val liftrel_def = Define`
+  liftrel b ty R x y = (if b then I else (~))
+                         ((case ty of Atomic -> I || TC -> TC)
+                          R x y)
+`;
+
+
 val eval_def = Define`
-  eval (Fa : 'n -> 'a -> 'a -> bool)
-       (G : 'n -> ('a + 'b) -> ('a + 'b) -> bool)
+  eval (Fa : ('n # 'a # 'a # bool # reltype) -> bool)
+       (G : ('n # ('a + 'b) # ('a + 'b) # bool # reltype) -> bool)
        (R : 'n -> 'c -> 'c -> bool) =
     ! (f : 'a -> 'c).
-         (!a1 a2 n. Fa n a1 a2 ==> R n (f a1) (f a2)) ==>
+         (!a1 a2 n b ty. (n, a1, a2, b, ty) IN Fa ==>
+                         liftrel b ty (R n) (f a1) (f a2)) ==>
          ? (g : 'b -> 'c).
-              (!a1 a2 n. G n (INL a1) (INL a2) ==> R n (f a1) (f a2)) /\
-              (!a b n. G n (INL a) (INR b) ==> R n (f a) (g b)) /\
-              (!a b n. G n (INR b) (INL a) ==> R n (g b) (f a)) /\
-              (!b1 b2 n. G n (INR b1) (INR b2) ==> R n (g b1) (g b2))
+             (!a1 a2 n b ty. (n, INL a1, INL a2, b, ty) IN G ==>
+                             liftrel b ty (R n) (f a1) (f a2)) /\
+             (!a b n p ty. (n, INL a, INR b, p, ty) IN G ==>
+                           liftrel p ty (R n) (f a) (g b)) /\
+             (!a b n p ty. (n, INR b, INL a, p, ty) IN G ==>
+                           liftrel p ty (R n) (g b) (f a)) /\
+             (!b1 b2 n b ty. (n, INR b1, INR b2, b, ty) IN G ==>
+                             liftrel b ty (R n) (g b1) (g b2))
 `;
+
+(* Some example diagrams *)
 
 val diamond_eval = store_thm(
   "diamond_eval",
-  ``eval (\i m n. (i = 0) /\ ((m = 0) /\ (n = 1) \/ (m = 0) /\ (n = 2)))
-         (\i m n. (i = 0) /\ ((m = INL 1) /\ (n = INR 0) \/
-                              (m = INL 2) /\ (n = INR 0)))
+  ``eval {(0,0,1,T,Atomic); (0,0,2,T,Atomic)}
+         {(0,INL 1,INR 0,T,Atomic); (0,INL 2,INR 0,T,Atomic)}
          R
      = diamond (R 0)``,
-  SRW_TAC [DNF_ss][diamond_def, eval_def, EQ_IMP_THM] THENL [
+  SRW_TAC [DNF_ss] [diamond_def, eval_def, EQ_IMP_THM, liftrel_def] THENL [
     FIRST_X_ASSUM (Q.SPEC_THEN `\n. if n = 0 then x
                                     else if n = 1 then y
                                     else z`
@@ -36,21 +54,34 @@ val diamond_eval = store_thm(
 
 val totality_eval = store_thm(
   "totality_eval",
-  ``eval (\i m n. F) (\i m n. (i = 0) /\ (m = (INL 0)) /\ (n = (INL 1)))
-         R =
-    !x y. R 0 x y``,
-  SRW_TAC [DNF_ss][eval_def, EQ_IMP_THM] THEN
+  ``eval {} {(0, INL 0, INL 1, T, Atomic)} R = !x y. R 0 x y``,
+  SRW_TAC [DNF_ss][eval_def, EQ_IMP_THM, liftrel_def] THEN
   FIRST_X_ASSUM (Q.SPEC_THEN `\i. if i = 0 then x else y` MP_TAC) THEN
   SRW_TAC [][]);
 
+val lopsided_TC_diamond = store_thm(
+  "lopsided_TC_diamond",
+  ``eval {(0,0,1,T,Atomic); (0,0,2,T,TC)}
+         {(0,INL 1,INR 0,T,TC); (0,INL 2,INR 0,T,TC)} R =
+    !x y z. R 0 x y /\ TC (R 0) x z ==>
+            ?u. TC (R 0) y u /\ TC (R 0) z u``,
+  SRW_TAC [DNF_ss][eval_def, EQ_IMP_THM, liftrel_def] THENL [
+    FIRST_X_ASSUM (Q.SPEC_THEN `\n. if n = 0 then x
+                                    else if n = 1 then y
+                                    else z`
+                   MP_TAC) THEN
+    SRW_TAC [DNF_ss][] THEN METIS_TAC [],
+    `?u. TC (R 0) (f 1) u /\ TC (R 0) (f 2) u` by METIS_TAC [] THEN
+    Q.EXISTS_TAC `K u` THEN SRW_TAC [][]
+  ]);
+
 val sequentialisation_eval = store_thm(
   "sequentialisation_eval",
-  ``eval (\i m n. (i = 0) /\ (m = 0) /\ (n = 1))
-         (\i m n. (i = 1) /\ (m = INL 0) /\ (n = INR 0) \/
-                  (i = 2) /\ (m = INR 0) /\ (n = INL 1))
+  ``eval {(0,0,1,T,Atomic)}
+         {(1,INL 0,INR 0,T,Atomic); (2,INR 0,INL 1,T,Atomic)}
          R =
     (!x y. R 0 x y ==> ?z. R 1 x z /\ R 2 z y)``,
-  SRW_TAC [DNF_ss][eval_def, EQ_IMP_THM] THENL [
+  SRW_TAC [DNF_ss][eval_def, EQ_IMP_THM,liftrel_def] THENL [
     FIRST_X_ASSUM (Q.SPEC_THEN `\n. if n = 0 then x else y` MP_TAC) THEN
     SRW_TAC [DNF_ss][] THEN METIS_TAC [],
     `?z. R 1 (f 0) z /\ R 2 z (f 1)` by METIS_TAC [] THEN
@@ -58,18 +89,17 @@ val sequentialisation_eval = store_thm(
   ]);
 
 val only_black_eq_T = prove(
-  ``eval (\i m n. (i = 0) /\ (m = INL 0) /\ (n = INL 0)) (\i m n. F) R' = T``,
+  ``eval Fa {} R' = T``,
   SRW_TAC [DNF_ss][eval_def]);
 
 val relationally_reflected = store_thm(
   "relationally_reflected",
-  ``eval (\i m n. (i = 0) /\ (m = 0) /\ (n = 1))
-         (\i m n. (i = 1) /\ (m = INR 0) /\ (n = INL 0) \/
-                  (i = 1) /\ (m = INR 1) /\ (n = INL 1) \/
-                  (i = 2) /\ (m = INR 0) /\ (n = INR 1))
+  ``eval {(0,0,1,T,Atomic)}
+         {(1,INR 0,INL 0,T,Atomic); (1,INR 1,INL 1,T,Atomic);
+          (2,INR 0,INR 1,T,Atomic)}
          R =
     (!x y. R 0 x y ==> ?u v. R 1 u x /\ R 1 v y /\ R 2 u v)``,
-  SRW_TAC [DNF_ss][eval_def, EQ_IMP_THM] THENL [
+  SRW_TAC [DNF_ss][eval_def, EQ_IMP_THM, liftrel_def] THENL [
     FIRST_X_ASSUM (Q.SPEC_THEN `\n. if n = 0 then x else y` MP_TAC) THEN
     SRW_TAC [DNF_ss][] THEN METIS_TAC [],
     `?u v. R 1 u (f 0) /\ R 1 v (f 1) /\ R 2 u v` by METIS_TAC [] THEN
@@ -77,56 +107,169 @@ val relationally_reflected = store_thm(
     SRW_TAC [][]
   ]);
 
-val Rhomo_def = Define`
-  Rhomo f R1 R2 = !x y. R1 x y ==> R2 (f x) (f y)
+val no_1step_join = store_thm(
+  "no_1step_join",
+  ``eval {(0,0,1,T,Atomic); (0,0,2,T,Atomic)}
+         {(0,INL 1,INL 2,F,Atomic)} R =
+    (!x y z. R 0 x y /\ R 0 x z ==> ~R 0 y z)``,
+  SRW_TAC [DNF_ss][eval_def, EQ_IMP_THM, liftrel_def] THENL [
+    FIRST_X_ASSUM (Q.SPEC_THEN `\n. if n = 0 then x
+                                    else if n = 1 then y else z` MP_TAC) THEN
+    SRW_TAC [DNF_ss][],
+    METIS_TAC []
+  ]);
+
+val no_terminal_object = store_thm(
+  "no_terminal_object",
+  ``eval {} {(0,INR 0,INL 0,F,Atomic)} R  = !y. ?x. ~R 0 x y``,
+  SRW_TAC [DNF_ss][eval_def, EQ_IMP_THM, liftrel_def] THENL [
+    FIRST_X_ASSUM (Q.SPEC_THEN `\n. y` MP_TAC) THEN SRW_TAC [][] THEN
+    METIS_TAC [],
+    `?u. ~R 0 u (f 0)` by METIS_TAC [] THEN
+    Q.EXISTS_TAC `\n. u` THEN SRW_TAC [][]
+  ]);
+
+(* ----------------------------------------------------------------------
+    Theory of diagram equivalence
+   ---------------------------------------------------------------------- *)
+
+
+(* basic concepts *)
+val Pres_def = Define`
+  Pres f R1 R2 = !x y. R1 x y ==> R2 (f x) (f y)
 `;
 
 val onto_def = Define`
   onto f = !x. ?y. f y = x
 `;
 
-val ARSh_def = Define`
-  ARSh f R1 R2 = (!b. ?a. f(a) = b) /\
-                 (!x y. R1 x y ==> R2 (f x) (f y))
-`;
-
-val ARSh_alt = store_thm(
-  "ARSh_alt",
-  ``ARSh f R1 R2 = onto f /\ Rhomo f R1 R2``,
-  SRW_TAC [][onto_def, Rhomo_def, ARSh_def]);
-
-val full_def = Define`
-  full f R1 R2 = !b1 b2. R2 b1 b2 ==>
+val sRefl_def = Define`
+  sRefl f R1 R2 = !b1 b2. R2 b1 b2 ==>
                          ?a1 a2. R1 a1 a2 /\ (b1 = f a1) /\ (b2 = f a2)
 `;
 
-val lrfull_def = Define`
-  lrfull f R1 R2 = !x y. R2 (f x) (f y) ==> R1 x y
+val aRefl_def = Define`
+  aRefl f R1 R2 = !x y. R2 (f x) (f y) ==> R1 x y
 `;
 
-val ARSh_RTC = store_thm(
-  "ARSh_RTC",
-  ``ARSh f R1 R2 ==> ARSh f (RTC R1) (RTC R2)``,
-  SRW_TAC [][ARSh_def] THEN
-  Q_TAC SUFF_TAC `!x y. RTC R1 x y ==> RTC R2 (f x) (f y)`
-        THEN1 METIS_TAC [] THEN
-  HO_MATCH_MP_TAC RTC_INDUCT THEN METIS_TAC [RTC_RULES]);
+val kCompl_def = Define`
+  kCompl s f = !x y. (f x = f y) ==> EQC s x y
+`;
 
-val skernel_def = Define`
-  skernel s f = !x y. (f x = f y) ==> EQC s x y
+val kSound_def = Define`
+  kSound s f = !x y. s x y ==> (f x = f y)
 `;
 
 val ofree_def = Define`
   ofree s = !x y. EQC s x y ==> RTC s x y
 `;
 
+val presrefl_atomic = store_thm(
+  "presrefl_atomic",
+  ``Pres f R1 R2 /\ aRefl f R1 R2 ==> !x y. R1 x y = R2 (f x) (f y)``,
+  SRW_TAC [][Pres_def, aRefl_def] THEN METIS_TAC []);
+
+val presrefl_TC = store_thm(
+  "presrefl_TC",
+  ``onto f /\ Pres f R1 R2 /\ aRefl f R1 R2 ==>
+    (!x y. TC R1 x y = TC R2 (f x) (f y))``,
+  SIMP_TAC (srw_ss()) [onto_def] THEN STRIP_TAC THEN
+  `!x y. R1 x y = R2 (f x) (f y)` by METIS_TAC [presrefl_atomic] THEN
+  SIMP_TAC (srw_ss() ++ DNF_ss) [EQ_IMP_THM] THEN CONJ_TAC THENL [
+    HO_MATCH_MP_TAC TC_INDUCT THEN METIS_TAC [TC_RULES],
+    Q_TAC SUFF_TAC `!a b. TC R2 a b ==> !x y. (a = f x) /\ (b = f y) ==>
+                                              TC R1 x y`
+          THEN1 METIS_TAC [] THEN
+    HO_MATCH_MP_TAC TC_INDUCT THEN
+    SRW_TAC [][] THENL [
+      METIS_TAC [TC_RULES],
+      `?a0. f a0 = a'` by METIS_TAC [] THEN
+      METIS_TAC [TC_RULES]
+    ]
+  ]);
+
+val presrefl_liftrel = store_thm(
+  "presrefl_liftrel",
+  ``onto f /\ Pres f R1 R2 /\ aRefl f R1 R2 ==>
+    !x y b ty. liftrel b ty R1 x y = liftrel b ty R2 (f x) (f y)``,
+  SRW_TAC [][liftrel_def] THEN
+  Cases_on `ty` THEN SRW_TAC [][presrefl_TC, presrefl_atomic]);
+
+val aRefl_TC = store_thm(
+  "aRefl_TC",
+  ``aRefl f R1 R2 /\ onto f ==> aRefl f (TC R1) (TC R2)``,
+  SIMP_TAC (srw_ss()) [aRefl_def, onto_def] THEN STRIP_TAC THEN
+  Q_TAC SUFF_TAC `!a b. TC R2 a b ==> !x y. (a = f x) /\ (b = f y) ==>
+                                            TC R1 x y`
+        THEN1 METIS_TAC [] THEN
+  HO_MATCH_MP_TAC TC_INDUCT THEN SRW_TAC [][] THEN
+  METIS_TAC [TC_RULES]);
+
+
+(* important theorem *)
+val diagram_preservation = store_thm(
+  "diagram_preservation",
+  ``!R1 R2 h.
+       onto h /\ (!n. Pres h (R1 n) (R2 n) /\ aRefl h (R1 n) (R2 n)) ==>
+       !Fa G. eval Fa G R1 = eval Fa G R2``,
+  REPEAT STRIP_TAC THEN
+  `!n a1 a2 b ty. liftrel b ty (R1 n) a1 a2 =
+                  liftrel b ty (R2 n) (h a1) (h a2)`
+     by METIS_TAC [presrefl_liftrel] THEN
+  `?invh. !b. h (invh b) = b` by METIS_TAC [SKOLEM_THM, onto_def] THEN
+  ASM_SIMP_TAC (srw_ss()) [eval_def] THEN EQ_TAC THEN REPEAT STRIP_TAC THENL [
+    FIRST_X_ASSUM (MP_TAC o SPEC ``(invh : 'c -> 'b) o (f : 'd -> 'c)``) THEN
+    SRW_TAC [][] THEN
+    Q.EXISTS_TAC `h o g` THEN SRW_TAC [][],
+
+    FIRST_X_ASSUM (MP_TAC o SPEC ``(h : 'b -> 'c) o (f : 'd -> 'b)``) THEN
+    SRW_TAC [][] THEN
+    Q.EXISTS_TAC `invh o g` THEN SRW_TAC [][]
+  ]);
+
+
+(* but aRefl is a strong requirement to make of a homomorphism...
+     (some might argue that onto is as well)
+   so let's try to weaken aRefl to sRefl.  We can do so by adding
+   structure *)
+
+val Refl_is_someany_with_structure = store_thm(
+  "Refl_is_someany_with_structure",
+  ``kSound s f /\ kCompl s f /\ onto f ==>
+    (sRefl f R1 R2 = aRefl f (EQC s O R1 O EQC s) R2)``,
+  SRW_TAC [][EQ_IMP_THM, kSound_def, kCompl_def, onto_def, sRefl_def,
+             aRefl_def]
+  THENL [
+    RES_TAC THEN SRW_TAC [][O_DEF] THEN METIS_TAC [],
+    `?a1 a2. (b1 = f a1) /\ (b2 = f a2)` by METIS_TAC [] THEN
+    SRW_TAC [][] THEN RES_TAC THEN
+    FULL_SIMP_TAC (srw_ss()) [O_DEF] THEN
+    Q_TAC SUFF_TAC `!x y. equiv_closure s x y ==> (f x = f y)`
+          THEN1 METIS_TAC [] THEN
+    HO_MATCH_MP_TAC EQC_INDUCTION THEN METIS_TAC []
+  ]);
+
+val Pres_ok_with_structure = store_thm(
+  "Pres_ok_with_structure",
+  ``kSound s f /\ Pres f R1 R2 ==> Pres f (EQC s O R1 O EQC s) R2``,
+  SRW_TAC [][Pres_def, kSound_def, O_DEF] THEN
+  Q_TAC SUFF_TAC `!x y. equiv_closure s x y ==> (f x = f y)` THEN1
+        METIS_TAC [] THEN
+  HO_MATCH_MP_TAC EQC_INDUCTION THEN METIS_TAC []);
+
+
+(* pre-order reduction *)
+
+(* paper's name for this theorem is
+     "Pre-ordered structural reflection is some/any"
+*)
 val note_lemma9 = store_thm(
   "note_lemma9",
-  ``onto f  /\ skernel s f /\ ofree s ==>
-    (full f (RTC (x RUNION s)) (RTC y) =
-     lrfull f (RTC (x RUNION s)) (RTC y))``,
-  SIMP_TAC (srw_ss()) [onto_def, skernel_def, ofree_def, full_def,
-                       lrfull_def] THEN STRIP_TAC THEN EQ_TAC
+  ``onto f  /\ kCompl s f /\ ofree s ==>
+    (sRefl f (RTC (x RUNION s)) (RTC y) =
+     aRefl f (RTC (x RUNION s)) (RTC y))``,
+  SIMP_TAC (srw_ss()) [onto_def, kCompl_def, ofree_def, sRefl_def,
+                       aRefl_def] THEN STRIP_TAC THEN EQ_TAC
   THENL [
     STRIP_TAC THEN MAP_EVERY Q.X_GEN_TAC [`a1`, `a2`] THEN STRIP_TAC THEN
     `?a1' a2'. RTC (x RUNION s) a1' a2' /\ (f a1' = f a1) /\ (f a2' = f a2)`
@@ -138,11 +281,14 @@ val note_lemma9 = store_thm(
     METIS_TAC []
   ]);
 
+(* paper's name for this theorem is
+     "Some-Reflection is Structurally Pre-ordered"
+*)
 val note_prop10_1 = store_thm(
   "note_prop10_1",
-  ``onto f /\ skernel s f /\ ofree s /\ full f x y ==>
-    full f (RTC (x RUNION s)) (RTC y)``,
-  SIMP_TAC (srw_ss()) [full_def, onto_def, ofree_def, skernel_def] THEN
+  ``onto f /\ kCompl s f /\ ofree s /\ sRefl f x y ==>
+    sRefl f (RTC (x RUNION s)) (RTC y)``,
+  SIMP_TAC (srw_ss()) [sRefl_def, onto_def, ofree_def, kCompl_def] THEN
   STRIP_TAC THEN
   HO_MATCH_MP_TAC RTC_INDUCT THEN CONJ_TAC THENL [
     METIS_TAC [chap3Theory.RUNION_RTC_MONOTONE, RUNION_COMM],
@@ -156,37 +302,12 @@ val note_prop10_1 = store_thm(
     METIS_TAC [RTC_RTC]
   ]);
 
-val diagram_preservation = store_thm(
-  "diagram_preservation",
-  ``!R1 R2 h.
-       onto h /\ (!n. Rhomo h (R1 n) (R2 n) /\ lrfull h (R1 n) (R2 n)) ==>
-       !Fa G. eval Fa G R1 = eval Fa G R2``,
-  SRW_TAC [][EQ_IMP_THM, onto_def, Rhomo_def, lrfull_def, eval_def] THEN
-  `?invh. !b. h (invh b) = b` by METIS_TAC [SKOLEM_THM] THENL [
-    `!g1 g2 n. Fa n g1 g2 ==> R1 n (invh (f g1)) (invh (f g2))`
-        by (REPEAT STRIP_TAC THEN
-            `R2 n (f g1) (f g2)` by METIS_TAC [] THEN
-            `(f g1 = h (invh (f g1))) /\ (f g2 = h (invh (f g2)))`
-                by SRW_TAC [][] THEN
-            METIS_TAC []) THEN
-    FIRST_X_ASSUM (MP_TAC o SPEC ``(invh : 'c -> 'b) o (f : 'd -> 'c)``) THEN
-    SRW_TAC [][] THEN
-    Q.EXISTS_TAC `h o g` THEN SRW_TAC [][] THEN METIS_TAC [],
-
-    FIRST_X_ASSUM (MP_TAC o SPEC ``(h : 'b -> 'c) o (f : 'd -> 'b)``) THEN
-    SRW_TAC [][] THEN
-    Q.EXISTS_TAC `invh o g` THEN SRW_TAC [][]
-  ]);
-
-val scollapse_def = Define`
-  scollapse s f = !x y. s x y ==> (f x = f y)
-`;
-
-val Rhomo_structure_RTC = store_thm(
-  "Rhomo_structure_RTC",
-  ``Rhomo f R1 R2 /\ scollapse s f ==>
-    Rhomo f (RTC (R1 RUNION s)) (RTC R2)``,
-  SIMP_TAC (srw_ss()) [Rhomo_def, scollapse_def] THEN STRIP_TAC THEN
+(* "structural pre-ordered preservation" *)
+val Pres_structure_RTC = store_thm(
+  "Pres_structure_RTC",
+  ``Pres f R1 R2 /\ kSound s f ==>
+    Pres f (RTC (R1 RUNION s)) (RTC R2)``,
+  SIMP_TAC (srw_ss()) [Pres_def, kSound_def] THEN STRIP_TAC THEN
   HO_MATCH_MP_TAC RTC_INDUCT THEN SRW_TAC [][RTC_RULES, RUNION] THEN
   METIS_TAC [RTC_RULES]);
 
